---
title: "L'Hospital's Rule"
---

# [L'Hospital's_Rule](/notes/areas/mathematics/real_analysis/definitions/lhospitals_rule/)

<div class="callout callout-warning">
<div class="callout-title"><span class="callout-icon">⚠️</span>AI-Generated</div>
<div class="callout-content">

This file was generated by AI and may require review.

</div>
</div>

## Definition

Assume $f$ and $g$ are [differentiable](/notes/areas/mathematics/real_analysis/definitions/differentiable/) on $(a,b)$ and that $g'(x) \neq 0$ for all $x \in (a,b)$. If



$$
\lim_{x \to a^+} f(x) = 0 \quad\text{and}\quad \lim_{x \to a^+} g(x) = 0
$$



then



$$
\lim_{x \to a^+} \frac{f(x)}{g(x)} = \lim_{x \to a^+} \frac{f'(x)}{g'(x)}
$$



provided the limit on the right-hand side exists.

The rule also applies to the indeterminate form $\frac{\infty}{\infty}$.

## Proof

By the [Generalized_Mean_Value_Theorem](/notes/areas/mathematics/real_analysis/definitions/generalized_mean_value_theorem/), for each $x \in (a,b)$ there exists $c_x$ between $a$ and $x$ such that



$$
\frac{f(x)}{g(x)} = \frac{f(x) - f(a)}{g(x) - g(a)} = \frac{f'(c_x)}{g'(c_x)}
$$



(using $f(a) = g(a) = 0$ by [continuity](/notes/areas/mathematics/real_analysis/definitions/continuity/)).

As $x \to a^+$, we have $c_x \to a^+$, so the result follows.
